improved comments in the encoding

theories/BI/Utils/encoding.v
@@ -21,229 +21,331 @@ Set Implicit Arguments.
 
 #[local] Notation "X ⊆ Y" := (∀m, X m → Y m) (at level 70).
 #[local] Infix "∊" := In (at level 70).
+
 #[local] Infix "~p" := (@Permutation _) (at level 70).
 
 #[local] Hint Constructors Permutation : core.
 
-Fact permutation_in_head {X} (x : X) l : x ∊ l → ∃m, l ~p x::m.
+#[local] Fact permutation_in_head {X} (x : X) l : x ∊ l → ∃m, l ~p x::m.
 Proof.
   induction l as [ | y l IHl ].
   + intros [].
   + intros [ <- | []%IHl ]; eauto.
 Qed.
 
-  Notation "x ≡ y" := (BI_bunch_equiv x y) (at level 70, no associativity, format "x  ≡  y").
-  Notation "C [ Δ ]" := (BI_ctx_fill C Δ) (at level 1, no associativity, format "C [ Δ ]").
+#[local] Notation "x ≡ y" := (BI_bunch_equiv x y) (at level 70, no associativity, format "x  ≡  y").
+#[local] Notation "C [ Δ ]" := (BI_ctx_fill C Δ) (at level 1, no associativity, format "C [ Δ ]").
 
-  Notation "⟨ A ⟩" := (BI_bunch_atom A) (at level 0, format "⟨ A ⟩"). 
-  Notation "'ø[' k ']'" := (BI_bunch_unit _ _ k) (at level 0, no associativity, format "ø[ k ]").
-  Notation "Γ '⊛[' k ']' Δ" := (BI_bunch_comp k Γ Δ) (at level 65, left associativity, format "Γ  ⊛[ k ]  Δ").
-  Notation øₐ := ø[BI_addi].
-  Notation øₘ := ø[BI_mult].
-  Notation "Γ '⊛ₐ' Δ" := (Γ ⊛[BI_addi] Δ) (at level 65, left associativity, format "Γ  ⊛ₐ  Δ").
-  Notation "Γ '⊛ₘ' Δ" := (Γ ⊛[BI_mult] Δ) (at level 65, left associativity, format "Γ  ⊛ₘ  Δ").
+#[local] Notation "⟨ A ⟩" := (BI_bunch_atom A) (at level 0, format "⟨ A ⟩"). 
+#[local] Notation "'ø[' k ']'" := (BI_bunch_unit _ _ k) (at level 0, no associativity, format "ø[ k ]").
+#[local] Notation "Γ '⊛[' k ']' Δ" := (BI_bunch_comp k Γ Δ) (at level 65, left associativity, format "Γ  ⊛[ k ]  Δ").
+#[local] Notation øₐ := ø[BI_addi].
+#[local] Notation øₘ := ø[BI_mult].
+#[local] Notation "Γ '⊛ₐ' Δ" := (Γ ⊛[BI_addi] Δ) (at level 65, left associativity, format "Γ  ⊛ₐ  Δ").
+#[local] Notation "Γ '⊛ₘ' Δ" := (Γ ⊛[BI_mult] Δ) (at level 65, left associativity, format "Γ  ⊛ₘ  Δ").
 
-  Notation "£ v" := (@BI_form_var _ _ v) (at level 1, format "£ v").
-  Notation "⊥" := (@BI_form_bot _ _ eq_refl).
-  Notation "1" := (@BI_form_unit _ _ BI_mult eq_refl).
-  Notation "A ⇒ B" := (@BI_form_impl _ _ BI_addi eq_refl A B) (at level 63, right associativity, format "A ⇒ B").
-  Notation "A '-∗' B" := (@BI_form_impl _ _ BI_mult eq_refl A B) (at level 63, right associativity, format "A -∗ B").
-  Notation "A ∗ B" := (@BI_form_conj _ _ BI_mult eq_refl A B) (at level 59, left associativity, format "A ∗ B").
-  Notation "A ⩑ B" := (@BI_form_conj _ _ BI_addi eq_refl A B) (at level 59, left associativity, format "A ⩑ B").
-  Notation "A ⩒ B" := (@BI_form_disj _ _ eq_refl A B) (at level 61, left associativity, format "A ⩒ B").
- 
+#[local] Notation "£ v" := (@BI_form_var _ _ v) (at level 1, format "£ v").
+#[local] Notation "⊥" := (@BI_form_bot _ _ eq_refl).
+#[local] Notation "1" := (@BI_form_unit _ _ BI_mult eq_refl).
+#[local] Notation "A ⇒ B" := (@BI_form_impl _ _ BI_addi eq_refl A B) (at level 63, right associativity, format "A ⇒ B").
+#[local] Notation "A '-∗' B" := (@BI_form_impl _ _ BI_mult eq_refl A B) (at level 63, right associativity, format "A -∗ B").
+#[local] Notation "A ∗ B" := (@BI_form_conj _ _ BI_mult eq_refl A B) (at level 59, left associativity, format "A ∗ B").
+#[local] Notation "A ⩑ B" := (@BI_form_conj _ _ BI_addi eq_refl A B) (at level 59, left associativity, format "A ⩑ B").
+#[local] Notation "A ⩒ B" := (@BI_form_disj _ _ eq_refl A B) (at level 61, left associativity, format "A ⩒ B").
+
 Arguments BI_ctx_hole {_ _}.
+
+#[local] Reserved Notation "'![' γ ']' φ" (at level 1, format "![ γ ] φ").
+#[local] Reserved Notation "Γ ⊦ A" (at level 70, no associativity, format "Γ  ⊦  A").
+#[local] Reserved Notation "⟦ A ⟧" (at level 0, format "⟦ A ⟧").
+
+(* The (-∗,⇒,⩑,1) fragment of LBI *)
+Definition BI_fragment_impl_conj_unit c :=
+  match c with
+  | BI_unit BI_mult => true   (* 1 *)
+  | BI_impl _       => true   (* -∗ and ⇒ *)
+  | BI_conj BI_addi => true   (* ⩑ *)
+  | _               => false  (* no other connective *)
+  end.
+
+#[local] Notation µ := BI_fragment_impl_conj_unit.
+
+#[local] Notation "⨂ₘ" := BI_list_mult.
+
+(* We work in cut-free fragments of LBI *)
+#[local] Notation "Γ ⊦ A" := (LBI_provable BI_cut_free Γ A).
 
 Section pseudo_exponential.
 
-  Definition µ (c : BI_conn) : bool :=
-    match c with
-    | BI_unit BI_mult => true
-    | BI_impl _       => true
-    | BI_conj BI_addi => true
-    | _ => false
-    end.
+  Variable (prop : Set).
 
-  Variables (prop : Set).
-
+  (* We work in the (-∗,⇒,⩑,1) fragment of BI *)
   Implicit Types (φ : BI_form µ prop) (Γ : BI_bunch µ prop).
 
+  (* We simulate ⊤ using 1⇒1 *)
   Notation "⊤" := (1⇒1).
 
+  (** This is the major breakthrought that allows for the encoding
+      of the dereliction rule in BI, see BI_pseudo_exp_derilection below *)
+
   Definition BI_pseudo_exp γ φ := (⊤-∗((φ-∗γ)⇒γ))⩑1.
+  Notation "![ γ ] φ" := (BI_pseudo_exp γ φ).
 
-  Notation "'![' γ ']' φ" := (BI_pseudo_exp γ φ) (at level 1, format "![ γ ] φ").
-  Notation "Γ ⊦ A" := (LBI_provable BI_cut_free Γ A) (at level 70, no associativity, format "Γ  ⊦  A").
+  (** We study the LBI proof theory of the pseudo-exponential ![γ]φ, 
+      restricted to the (-∗,⇒,⩑,1) cut-free fragment of LBI. *)
 
-  Fact BI_unit_right_l k Γ γ : Γ ⊦ γ → ø[k] ⊛[k] Γ ⊦ γ.
-  Proof. apply BI_sp_equiv, BI_bequiv_sym, BI_bequiv_neut. Qed.
+  (** First some tools to facilitate LBI proofs *)
 
-  Fact BI_unit_left_r k Γ γ : Γ ⊛[k] ø[k] ⊦ γ → Γ ⊦ γ.
+  Local Fact BI_unit_right_l k Γ γ :
+             Γ ⊦ γ 
+    → (*-----------------*)
+         ø[k] ⊛[k] Γ ⊦ γ.
   Proof.
-    apply BI_sp_equiv.
-    apply BI_bequiv_trans with (1 := BI_bequiv_comm _ _ _), BI_bequiv_neut.
+    apply BI_sp_equiv,
+          BI_bequiv_sym,
+          BI_bequiv_neut.
   Qed.
 
-  Fact BI_top_weak Γ : Γ ⊦ ⊤.
+  Local Fact BI_unit_left_r k Γ γ :
+          Γ ⊛[k] ø[k] ⊦ γ
+    →  (*-----------------*)
+             Γ ⊦ γ.
+  Proof.
+    apply BI_sp_equiv,
+          BI_bequiv_trans with (1 := BI_bequiv_comm _ _ _),
+          BI_bequiv_neut.
+  Qed.
+
+  Local Fact BI_top_weak Γ : Γ ⊦ ⊤.
   Proof.
     change (BI_ctx_hole[Γ] ⊦ ⊤).
-    apply BI_sp_weak, BI_sp_impl_r, BI_unit_right_l, BI_sp_axiom.
+    apply BI_sp_weak,
+          BI_sp_impl_r,
+          BI_unit_right_l,
+          BI_sp_axiom.
   Qed.
 
-  Fact BI_cntr_all Γ γ : Γ ⊛ₐ Γ ⊦ γ → Γ ⊦ γ.
+  Local Fact BI_cntr_all Γ γ : Γ ⊛ₐ Γ ⊦ γ → Γ ⊦ γ.
   Proof.
     intro.
     change (BI_ctx_hole[Γ] ⊦ γ).
     now apply BI_sp_cntr.
   Qed.
 
-  Fact BI_simpl_imp_l Γ A B C : Γ ⊦ A → ⟨B⟩ ⊦ C → Γ ⊛ₐ ⟨A⇒B⟩ ⊦ C.
+  Local Fact BI_simpl_imp_l Γ A B C :
+          Γ ⊦ A    →     ⟨B⟩ ⊦ C
+    →  (*------------------------*)
+             Γ ⊛ₐ ⟨A⇒B⟩ ⊦ C.
   Proof. apply BI_sp_impl_l with (Γ := BI_ctx_hole). Qed.
 
-  Fact BI_simpl_wand_l Γ A B C : Γ ⊦ A → ⟨B⟩ ⊦ C → Γ ⊛ₘ ⟨A-∗B⟩ ⊦ C.
+  Local Fact BI_simpl_wand_l Γ A B C :
+          Γ ⊦ A    →     ⟨B⟩ ⊦ C
+    →  (*------------------------*)
+             Γ ⊛ₘ ⟨A-∗B⟩ ⊦ C.
   Proof. apply BI_sp_impl_l with (Γ := BI_ctx_hole). Qed.
 
-  Lemma BI_pseudo_exp_weak Γ γ φ ψ :
+  (** Now the "weakening" rule for ![γ]φ *)
+
+  Proposition BI_pseudo_exp_weak Γ γ φ ψ :
              Γ ⊦ ψ 
       (*------------------*)
     →    Γ ⊛ₘ ⟨![γ]φ⟩ ⊦ ψ.
   Proof.
     intros H.
-    set (Δ := BI_ctx_comp BI_left BI_mult Γ BI_ctx_hole).
-    change (Δ[⟨![γ]φ⟩] ⊦ ψ).
+
+    set (Σ := BI_ctx_comp BI_left BI_mult Γ BI_ctx_hole).
+    change (Σ[⟨![γ]φ⟩] ⊦ ψ).
     apply BI_sp_conj_l.
-    set (Δ' := BI_ctx_comp BI_left BI_mult Γ (BI_ctx_comp BI_right BI_addi ⟨1⟩ BI_ctx_hole)).
-    change (Δ'[⟨⊤-∗(φ-∗γ)⇒γ⟩] ⊦ ψ).
+
+    set (Σ' := BI_ctx_comp BI_left BI_mult Γ (BI_ctx_comp BI_right BI_addi ⟨1⟩ BI_ctx_hole)).
+    change (Σ'[⟨⊤-∗(φ-∗γ)⇒γ⟩] ⊦ ψ).
     apply BI_sp_weak.
-    change (Δ[øₐ ⊛ₐ ⟨1⟩] ⊦ ψ).
-    apply BI_sp_equiv with Δ[⟨1⟩].
+
+    change (Σ[øₐ ⊛ₐ ⟨1⟩] ⊦ ψ).
+    apply BI_sp_equiv with Σ[⟨1⟩].
     1: apply BI_bequiv_congr, BI_bequiv_sym, BI_bequiv_neut.
+
     apply BI_sp_unit_l.
     simpl.
+
     revert H; apply BI_sp_equiv.
     apply BI_bequiv_sym,
           BI_bequiv_trans with (1 := BI_bequiv_comm _ _ _),
           BI_bequiv_neut.
   Qed.
 
-  Theorem BI_list_mult_weak Σ Γ ψ :
-      (∀A, A ∊ Σ → ∃ γ φ, A = ![γ]φ)
-    → Γ ⊦ ψ 
-    → (BI_list_mult Σ) ⊛ₘ Γ ⊦ ψ.
+  Check BI_pseudo_exp_weak.
+
+  (* We generalize the weakening rule to lists of ![γ]φ 
+
+     Notice that ⨂ₘ[A₁;...;Aₙ] := A₁ ⊛ₘ (... ⊛ₘ (Aₙ ⊛ₘ 1)...) *)
+  Lemma BI_list_mult_weak Σ Γ ψ (HΣ : ∀A, A ∊ Σ → ∃ γ φ, A = ![γ]φ) :
+             Γ ⊦ ψ 
+    →  (*---------------*)
+          ⨂ₘ Σ ⊛ₘ Γ ⊦ ψ.
   Proof.
-    intros H1%Forall_forall H; revert H1.
-    induction 1 as [ | A Σ (γ & φ & ->) _ IH ]; simpl.
-    + revert H; apply BI_sp_equiv.
-      apply BI_bequiv_sym, BI_bequiv_neut.
+    rewrite <- Forall_forall in HΣ.
+    intros H.
+    induction HΣ as [ | A Σ (γ & φ & ->) _ IH ]; simpl.
+    + revert H.
+      apply BI_sp_equiv,
+            BI_bequiv_sym,
+            BI_bequiv_neut.
     + apply BI_sp_equiv with (1 := BI_bequiv_sym (BI_bequiv_assoc _ _ _ _)),
             BI_sp_equiv with (1 := BI_bequiv_comm _ _ _),
             BI_pseudo_exp_weak; trivial.
   Qed.
 
-  Fact BI_first_idea Γ γ φ : Γ ⊛ₘ ⟨φ⟩ ⊦ γ → Γ ⊛ₐ ⟨(φ-∗γ)⇒γ⟩ ⊦ γ.
+  (** Now we explain the "dereliction" rule as the combination of
+      two ideas 1) & 2), leading to 3) when combined:
+      1) recover φ in multiplicative context 
+         from φ-∗γ)⇒γ in additive context
+      2) extract of "copy" of φ in additive context 
+         from (⊤-∗φ)⩑1 in multiplicative context
+      3) Hence combined, we can extract a copy in multiplicative
+         context. *)
+
+  Local Proposition BI_first_idea Γ γ φ :
+            Γ ⊛ₘ ⟨φ⟩ ⊦ γ
+    → (*---------------------*)
+         Γ ⊛ₐ ⟨(φ-∗γ)⇒γ⟩ ⊦ γ.
   Proof.
-    intros H.
+    intro.
     apply BI_simpl_imp_l.
     + now apply BI_sp_impl_r.
     + simpl; apply BI_sp_axiom.
   Qed.
 
-  Fact BI_second_idea Γ γ φ :
-    (Γ ⊛ₘ ⟨(⊤-∗φ)⩑1⟩) ⊛ₐ ⟨φ⟩ ⊦ γ → Γ ⊛ₘ ⟨(⊤-∗φ)⩑1⟩ ⊦ γ.
+  Local Proposition BI_second_idea Γ γ φ :
+         (Γ ⊛ₘ ⟨(⊤-∗φ)⩑1⟩) ⊛ₐ ⟨φ⟩ ⊦ γ
+    → (*------------------------------*)
+            Γ ⊛ₘ ⟨(⊤-∗φ)⩑1⟩ ⊦ γ.
   Proof.
     set (Δ := Γ ⊛ₘ ⟨(⊤-∗φ)⩑1⟩).
     intros H.
     apply BI_cntr_all.
     unfold Δ at 2.
-    set (Δ' := BI_ctx_comp BI_left BI_addi Δ
-              (BI_ctx_comp BI_left BI_mult Γ BI_ctx_hole)).
-    change (Δ'[⟨(⊤-∗φ)⩑1⟩] ⊦ γ).
+
+    set (Σ := BI_ctx_comp BI_left BI_addi Δ
+             (BI_ctx_comp BI_left BI_mult Γ BI_ctx_hole)).
+    change (Σ[⟨(⊤-∗φ)⩑1⟩] ⊦ γ).
     apply BI_sp_conj_l.
-    set (Δ'' := BI_ctx_comp BI_left BI_addi Δ
-               (BI_ctx_comp BI_left BI_mult Γ 
-               (BI_ctx_comp BI_left BI_addi ⟨⊤-∗φ⟩
-                BI_ctx_hole))).
-    change (Δ''[⟨1⟩] ⊦ γ).
+    simpl.
+
+    set (Σ' := BI_ctx_comp BI_left BI_addi Δ
+              (BI_ctx_comp BI_left BI_mult Γ 
+              (BI_ctx_comp BI_left BI_addi ⟨⊤-∗φ⟩
+               BI_ctx_hole))).
+    change (Σ'[⟨1⟩] ⊦ γ).
     apply BI_sp_weak.
-    change (Δ'[⟨⊤-∗φ⟩ ⊛ₐ øₐ] ⊦ γ).
-    apply BI_sp_equiv with (Δ'[⟨⊤-∗φ⟩]).
-    1: apply BI_bequiv_congr, BI_bequiv_congr, BI_bequiv_sym,
+    simpl.
+
+    change (Σ[⟨⊤-∗φ⟩ ⊛ₐ øₐ] ⊦ γ).
+    apply BI_sp_equiv with (Σ[⟨⊤-∗φ⟩]).
+    1: apply BI_bequiv_congr,
+             BI_bequiv_congr,
+             BI_bequiv_sym,
              BI_bequiv_trans with (1 := BI_bequiv_comm _ _ _),
              BI_bequiv_neut.
-    set (Δ''' := BI_ctx_comp BI_left BI_addi Δ BI_ctx_hole).
-    change (Δ'''[Γ ⊛ₘ ⟨⊤-∗φ⟩] ⊦ γ).
+    simpl.
+
+    set (Σ'' := BI_ctx_comp BI_left BI_addi Δ BI_ctx_hole).
+    change (Σ''[Γ ⊛ₘ ⟨⊤-∗φ⟩] ⊦ γ).
     apply BI_sp_impl_l; auto.
+
     apply BI_top_weak.
   Qed.
 
-  Lemma BI_pseudo_exp_derilection Γ γ φ :
+  Proposition BI_pseudo_exp_derilection Γ γ φ :
           Γ ⊛ₘ ⟨![γ]φ⟩ ⊛ₘ ⟨φ⟩ ⊦ γ
-        (*-----------------------*)
-    →        Γ ⊛ₘ ⟨![γ]φ⟩ ⊦ γ.
+    →  (*-------------------------*)
+            Γ ⊛ₘ ⟨![γ]φ⟩ ⊦ γ.
   Proof.
-    intros H.
+    intro.
     unfold BI_pseudo_exp.
     apply BI_second_idea.
     apply BI_first_idea.
     trivial.
   Qed.
 
-  Check BI_pseudo_exp_weak.
   Check BI_pseudo_exp_derilection.
 
-  Theorem BI_list_mult_derilection Σ γ φ :
-      ![γ]φ ∊ Σ
-    → (BI_list_mult Σ) ⊛ₘ ⟨φ⟩ ⊦ γ 
-    → (BI_list_mult Σ) ⊦ γ.
+  (* We generalize the dereliction rule to lists 
+     containing a pseudo exponential ![γ]φ *)
+
+  Lemma BI_list_mult_derilection Σ γ φ (HΣ : ![γ]φ ∊ Σ) :
+         ⨂ₘ Σ ⊛ₘ ⟨φ⟩ ⊦ γ 
+    → (*-----------------*)
+           ⨂ₘ Σ ⊦ γ.
   Proof.
-    intros (Σ' & H'%BI_list_mult_perm_bequiv)%permutation_in_head H.
+    revert HΣ; intros (Σ' & H'%BI_list_mult_perm_bequiv)%permutation_in_head H.
     apply BI_sp_equiv with (1 := BI_bequiv_sym H').
     simpl.
     apply BI_sp_equiv with (1 := BI_bequiv_comm _ _ _).
     apply BI_pseudo_exp_derilection.
     revert H; apply BI_sp_equiv.
-    do 2 apply BI_bequiv_sym, BI_bequiv_trans with (1 := BI_bequiv_comm _ _ _).
-    apply BI_bequiv_congr.
-    apply BI_bequiv_trans with (1 := H'), BI_bequiv_comm.
+    do 2 apply BI_bequiv_sym,
+               BI_bequiv_trans with (1 := BI_bequiv_comm _ _ _).
+    apply BI_bequiv_congr,
+          BI_bequiv_trans with (1 := H'),
+          BI_bequiv_comm.
   Qed.
 
-  Check BI_list_mult_weak.
-  Check BI_list_mult_derilection.
+  (** Now we recall the encoding of 2-ACM counter machines,
+      (ie with FORK, INC, DEC and STOP but no zero test)
+      in the (⩑,-∗) linear fragment of BI. *)
 
-  Fact BI_FORK Γ φ ψ γ : Γ ⊦ φ → Γ ⊦ ψ → Γ ⊛ₘ ⟨(φ⩑ψ)-∗γ⟩ ⊦ γ.
+  Local Fact BI_FORK Γ φ ψ γ :
+         Γ ⊦ φ    →    Γ ⊦ ψ 
+    → (*---------------------*)
+         Γ ⊛ₘ ⟨(φ⩑ψ)-∗γ⟩ ⊦ γ.
   Proof.
-    intros H1 H2.
+    intros.
     apply BI_simpl_wand_l.
     + now apply BI_cntr_all, BI_sp_conj_r.
     + apply BI_sp_axiom.
   Qed.
 
-  Fact BI_INC Γ φ ψ γ : Γ ⊛ₘ ⟨φ⟩ ⊦ ψ → Γ ⊛ₘ ⟨(φ-∗ψ)-∗γ⟩ ⊦ γ.
+  Local Fact BI_INC Γ φ ψ γ :
+             Γ ⊛ₘ ⟨φ⟩ ⊦ ψ
+    → (*----------------------*)
+         Γ ⊛ₘ ⟨(φ-∗ψ)-∗γ⟩ ⊦ γ.
   Proof.
-    intros H.
+    intros.
     apply BI_simpl_wand_l.
     + now apply BI_sp_impl_r.
     + apply BI_sp_axiom.
   Qed.
 
-  Fact BI_DEC Γ φ ψ γ : Γ ⊦ ψ → Γ ⊛ₘ ⟨φ⟩ ⊛ₘ ⟨φ-∗ψ-∗γ⟩ ⊦ γ.
+  Local Fact BI_DEC Γ φ ψ γ :
+                Γ ⊦ ψ
+    → (*---------------------------*)
+         Γ ⊛ₘ ⟨φ⟩ ⊛ₘ ⟨φ-∗ψ-∗γ⟩ ⊦ γ.
   Proof.
     intros H.
     apply BI_sp_equiv with (1 := BI_bequiv_sym (BI_bequiv_assoc _ _ _ _)).
-    set (Δ := BI_ctx_comp BI_left BI_mult Γ BI_ctx_hole).
-    change (Δ[⟨φ⟩ ⊛ₘ ⟨φ-∗ψ-∗γ⟩] ⊦ γ).
+
+    set (Σ := BI_ctx_comp BI_left BI_mult Γ BI_ctx_hole).
+    change (Σ[⟨φ⟩ ⊛ₘ ⟨φ-∗ψ-∗γ⟩] ⊦ γ).
     apply BI_sp_impl_l with (1 := BI_sp_axiom _ _).
     simpl.
+
     apply BI_simpl_wand_l; auto.
     apply BI_sp_axiom.
   Qed.
 
-  Fact BI_STOP Γ γ : Γ ⊦ 1 → Γ ⊛ₘ ⟨1-∗γ⟩ ⊦ γ.
+  Local Fact BI_STOP Γ γ :
+              Γ ⊦ 1
+    → (*-----------------*)
+         Γ ⊛ₘ ⟨1-∗γ⟩ ⊦ γ.
   Proof.
     intros.
     apply BI_simpl_wand_l; auto.
     apply BI_sp_axiom.
   Qed.
+
+  (** We finish with study the TPS semantics 
+      of the pseudo-exponential ![γ]φ *)
 
   Variables (M : Type) (plus : M → M → M) (e : M)
             (neut : ∀x, plus e x = x)
@@ -252,9 +354,11 @@ Section pseudo_exponential.
 
             (s : prop → M → Prop).
 
-  Notation "⟦ A ⟧" := (tps_BI_form plus e s A) (at level 0, format "⟦ A ⟧").
+  Notation "⟦ A ⟧" := (tps_BI_form plus e s A).
 
-  Theorem tps_BI_pseudo_exp γ φ : ⟦φ⟧ e → ∀x, ⟦BI_pseudo_exp γ φ⟧ x ↔ e = x.
+  (* Semantically, ![γ]φ behaves much like φ⩑1 wrt TPS, hence
+     irrelevant of the choice of γ *)
+  Proposition tps_BI_pseudo_exp γ φ : ⟦φ⟧ e → ∀x, ⟦![γ]φ⟧ x ↔ e = x.
   Proof using comm neut.
     intros Hφ x; split.
     1: intros []; auto.
@@ -281,36 +385,56 @@ Section ACM2_to_BI.
     | FORKₐ p q r => p
     end.
 
+  (** We start from a list of instructions Σ
+      and a list of location over approximating
+      the source location of instructions 
+      occuring in Σ *)
+
   Variables (Σ : list (@acm2_instr loc))
             (l : list loc)
             (HΣl : ∀i, i ∊ Σ → acm2_instr_src i ∊ l).
 
-  (** Encode 
+  (** This is a "positive" encoding of 2-ACM in
+      the (⩑,-∗) linear fragment of ILL/BI
         FORKₐ p q r --> q⩑r -∗ p
-        INCₐ b p q  --> (b -∗ q) -∗ p
-        DECₐ b p q  --> b -∗ q -∗ p
-        STOPₐ p     --> 1 -∗ p 
-   *)
+        INCₐ α p q  --> (α -∗ q) -∗ p
+        DECₐ β p q  --> β -∗ q -∗ p
+        STOPₐ p     --> 1 -∗ p
 
-  Definition acm2_instr_to_BI i : BI_form µ (loc+bool) :=
-    match i with
-    | STOPₐ p     => 1 -∗ £(inl p)
-    | INCₐ b p q  => (£(inr b) -∗ £(inl q)) -∗ £(inl p)
-    | DECₐ b p q  => £(inr b) -∗ £(inl q) -∗ £(inl p)
-    | FORKₐ p q r => (£(inl q) ⩑ £(inl r)) -∗ £(inl p)
-    end.
+      Notice that locations in loc are encoded into
+      variables in the left part of loc+bool
+      while the right part is used from the two
+      counters α/β *)
 
   Notation α := true.
   Notation β := false.
 
-  Definition acm2_ctx_to_BI x y := 
-       repeat £(inr α) x ++ repeat £(inr β) y 
-    ++ flat_map (fun p => map (fun i => BI_pseudo_exp £(inl p) (acm2_instr_to_BI i)) Σ) l.
+  Definition acm2_instr_to_BI i : BI_form µ (loc+bool) :=
+    match i with
+    | FORKₐ p q r => (£(inl q) ⩑ £(inl r)) -∗ £(inl p)
+    | INCₐ c p q  => (£(inr c) -∗ £(inl q)) -∗ £(inl p)
+    | DECₐ c p q  => £(inr c) -∗ £(inl q) -∗ £(inl p)
+    | STOPₐ p     => 1 -∗ £(inl p)
+    end.
 
-  Fact In_acm2_ctx_to_BI x y i p :
-        i ∊ Σ 
-     -> p = acm2_instr_src i
-     -> BI_pseudo_exp £(inl p) (acm2_instr_to_BI i) ∊ acm2_ctx_to_BI x y.
+  Notation encᵢ := acm2_instr_to_BI.
+
+  Notation "![ γ ] φ" := (BI_pseudo_exp γ φ).
+
+  Definition acm2_ctx_to_BI x y := 
+       repeat £(inr α) x
+    ++ repeat £(inr β) y 
+    ++ flat_map (λ p, map (λ i, ![£(inl p)](encᵢ i)) Σ) l.
+
+  Notation enc := acm2_ctx_to_BI.
+
+  (* enc x y collects all encodings of instruction 
+     ![p](encᵢ i) for any location that might occur
+     in any computation *)
+  Local Fact In_acm2_ctx_to_BI x y i p :
+      i ∊ Σ 
+    → p = acm2_instr_src i
+    → ![£(inl p)](encᵢ i) ∊ enc x y.
   Proof using HΣl.
     intros H1 H2.
     unfold acm2_ctx_to_BI; rewrite !in_app_iff, in_flat_map; do 2 right.
@@ -318,33 +442,37 @@ Section ACM2_to_BI.
     apply in_map_iff; eauto.
   Qed.
 
-  Fact acm2_ctx_to_BI_x x y Δ : 
-      BI_list_mult (acm2_ctx_to_BI (1+x) y) ⊛ₘ Δ 
-    ≡ BI_list_mult (acm2_ctx_to_BI x y) ⊛ₘ ⟨£(inr α)⟩ ⊛ₘ Δ.
+  (** enc x y also contains x copies of £α and y copies of £β *)
+
+  Local Fact acm2_ctx_to_BI_x x y Δ : 
+    ⨂ₘ (enc (1+x) y) ⊛ₘ Δ ≡ ⨂ₘ (enc x y) ⊛ₘ ⟨£(inr α)⟩ ⊛ₘ Δ.
   Proof. 
     do 2 apply BI_bequiv_trans with (1 := BI_bequiv_comm _ _ _), BI_bequiv_sym.
     apply BI_bequiv_congr, BI_bequiv_comm.
   Qed.
 
-  Fact acm2_ctx_to_BI_y x y Δ : 
-      BI_list_mult (acm2_ctx_to_BI x (1+y)) ⊛ₘ Δ 
-    ≡ BI_list_mult (acm2_ctx_to_BI x y) ⊛ₘ ⟨£(inr β)⟩ ⊛ₘ Δ.
+  Local Fact acm2_ctx_to_BI_y x y Δ : 
+    ⨂ₘ (enc x (1+y)) ⊛ₘ Δ ≡ ⨂ₘ (enc x y) ⊛ₘ ⟨£(inr β)⟩ ⊛ₘ Δ.
   Proof. 
-    do 2 apply BI_bequiv_trans with (1 := BI_bequiv_comm _ _ _), BI_bequiv_sym.
-    apply BI_bequiv_congr.
-    apply BI_bequiv_sym, 
+    do 2 apply BI_bequiv_trans with (1 := BI_bequiv_comm _ _ _),
+               BI_bequiv_sym.
+    apply BI_bequiv_congr,
+          BI_bequiv_sym, 
           BI_bequiv_trans with (1 := BI_list_mult_snoc _ _),
-          BI_list_mult_perm_bequiv.
-    unfold acm2_ctx_to_BI.
-    apply perm_trans with (2 := Permutation_app_swap_app _ _ _).
-    simpl; apply perm_skip, Permutation_app_swap_app.
+          BI_list_mult_perm_bequiv,
+          perm_trans with (2 := Permutation_app_swap_app _ _ _),
+          perm_skip,
+          Permutation_app_swap_app.
   Qed.
 
   Hint Resolve In_acm2_ctx_to_BI : core.
 
-  Lemma acm2_encode_sound x y p :
+  (** We can now show that our positive encoding is sound
+      wrt to cut-free provability in the (-∗,⇒,⩑,1) fragment *)
+
+  Local Lemma acm2_encode_sound x y p :
       acm2_accept Σ x y p
-    → LBI_provable BI_cut_free (BI_list_mult (acm2_ctx_to_BI x y)) £(inl p).
+    → ⨂ₘ (enc x y) ⊦ £(inl p).
   Proof using HΣl.
     induction 1 as [ p H 
                    | x y p q r H _ IH1 _ IH2
@@ -354,11 +482,13 @@ Section ACM2_to_BI.
                    | 
                    ];
         match goal with
-        | _ : ?i ∊ Σ |- _ => apply BI_list_mult_derilection with (φ := acm2_instr_to_BI i)
+        | _ : ?i ∊ Σ |- _ => apply BI_list_mult_derilection
+                               with (φ := acm2_instr_to_BI i)
         end; auto; simpl acm2_instr_to_BI.
     + apply BI_STOP.
       unfold acm2_ctx_to_BI; simpl.
-      apply BI_unit_left_r with (k := BI_mult), BI_list_mult_weak.
+      apply BI_unit_left_r with (k := BI_mult),
+            BI_list_mult_weak.
       2: apply BI_sp_unit_r.
       intros A; rewrite in_flat_map.
       intros (k & ? & (i & <- & ?)%in_map_iff); eauto.
@@ -374,8 +504,9 @@ Section ACM2_to_BI.
             BI_bequiv_trans with (1 := BI_list_mult_snoc _ _),
             BI_list_mult_perm_bequiv.
       unfold acm2_ctx_to_BI.
-      apply perm_trans with (2 := Permutation_app_swap_app _ _ _).
-      simpl; apply perm_skip, Permutation_app_swap_app.
+      apply perm_trans with (2 := Permutation_app_swap_app _ _ _),
+            perm_skip,
+            Permutation_app_swap_app.
     + apply BI_sp_equiv with (1 := BI_bequiv_sym (acm2_ctx_to_BI_x _ _ _)).
       now apply BI_DEC.
     + apply BI_sp_equiv with (1 := BI_bequiv_sym (acm2_ctx_to_BI_y _ _ _)).
@@ -384,6 +515,11 @@ Section ACM2_to_BI.
 
   Section completeness.
 
+    (** For the completeness, we use the soundness of
+        TPS semantics for LBI. We use nat² as a model
+        where (x,y) in nat² represents the value of
+        α/β. *)
+
     Let s (v : loc + bool) :=
       match v with
       | inl p => fun '(x,y) => acm2_accept Σ x y p
@@ -391,11 +527,12 @@ Section ACM2_to_BI.
       | inr β => eq (0,1)%nat
       end.
 
-    Notation sem := (tps_BI_form pair_add (0,0) s).
+    Notation "⟦ A ⟧" := (tps_BI_form pair_add (0,0) s A).
 
     Hint Constructors acm2_accept : core.
 
-    Local Lemma sem_complete_instr i : In i Σ -> sem (acm2_instr_to_BI i) (0, 0).
+    (* the semantics of instructions contains the unit of nat² *)
+    Local Lemma tps_instr_sound i : i ∊ Σ → ⟦encᵢ i⟧ (0,0).
     Proof.
       intros Hi.
       destruct i as [ | [] p q | [] p q | ]; simpl.
@@ -413,34 +550,39 @@ Section ACM2_to_BI.
       + intros [] []; rewrite pair_add_zero_right; eauto.
     Qed.
 
-    Variables (x y : nat) (p : loc)
-              (H : LBI_provable BI_cut_free (BI_list_mult (acm2_ctx_to_BI x y)) £(inl p)).
+    Variables (x y : nat) (p : loc) (Hxyp : ⨂ₘ (enc x y) ⊦ £(inl p)).
 
     Hint Resolve pair_add_zero_left pair_add_comm pair_add_assoc : core.
 
     Lemma acm2_encode_complete : acm2_accept Σ x y p.
-    Proof using H.
-      apply tps_LBI_sound with (plus := pair_add) (e := (0,0)) (s := s) (m := (x,y)) in H; auto.
-      apply tps_BI_equiv with (BI_list_mult (repeat £(inr α) x)
-                            ⊛ₘ (BI_list_mult (repeat £(inr β) y) 
-                            ⊛ₘ BI_list_mult (flat_map (fun p => map (fun i => BI_pseudo_exp £(inl p) (acm2_instr_to_BI i)) Σ) l)));
+    Proof using Hxyp.
+      (* TPS is sound for LBI *)
+      apply tps_LBI_sound with (plus := pair_add) (e := (0,0)) (s := s) (m := (x,y)) in Hxyp; auto.
+      (* We reorder ⨂ₘ (enc x y) *)
+      apply tps_BI_equiv with (⨂ₘ (repeat £(inr α) x)
+                           ⊛ₘ (⨂ₘ (repeat £(inr β) y) 
+                           ⊛ₘ  ⨂ₘ (flat_map (λ p, map (λ i, ![£(inl p)](encᵢ i)) Σ) l)));
         auto.
-      + unfold acm2_ctx_to_BI.
-        do 2 apply BI_bequiv_trans with (1 := BI_list_mult_app _ _), BI_bequiv_congr.
-        apply BI_bequiv_refl.
-      + exists (x,0), (0,y); split; simpl; auto; split.
-        * clear H.
-          induction x as [ | n IHn ]; simpl; auto.
+      + (* This is a reordering *)
+        do 2 apply BI_bequiv_trans with (1 := BI_list_mult_app _ _),
+                   BI_bequiv_congr; auto using BI_bequiv_refl.
+      + (* (x,0) belongs to ⟦⨂ₘ (repeat £(inr α) x)⟧
+           (0,y) belongs to ⟦⨂ₘ (repeat £(inr β) y)⟧
+           (0,0) belongs to the rest
+           so there sum (x,y) belongs to the semantics of this bunch *)
+        exists (x,0), (0,y); split; simpl; auto; split;
+          [ | exists (0,y), (0,0); split; simpl; auto; split ].
+        * clear Hxyp.
+          induction x as [ | n ]; simpl; auto.
           exists (1,0)%nat, (n,0); auto.
-        * exists (0,y), (0,0); split; simpl; auto; split.
-          - clear H.
-            induction y as [ | n IHn ]; simpl; auto.
-            exists (0,1)%nat, (0,n); auto.
-          - apply tps_BI_bunch_list_mult; auto.
-            intros A; rewrite in_flat_map.
-            intros (k & ? & (i & <- & ?)%in_map_iff).
-            apply tps_BI_pseudo_exp; auto.
-            now apply sem_complete_instr.
+        * clear Hxyp.
+          induction y as [ | n ]; simpl; auto.
+          exists (0,1)%nat, (0,n); auto.
+        * apply tps_BI_bunch_list_mult; auto.
+          intro; rewrite in_flat_map.
+          intros (? & ? & (? & <- & ?)%in_map_iff).
+          apply tps_BI_pseudo_exp; auto.
+          now apply tps_instr_sound.
     Qed.
 
   End completeness.
@@ -449,7 +591,7 @@ End ACM2_to_BI.
 
 #[local] Hint Resolve acm2_encode_sound acm2_encode_complete in_map : core.
 
-(** This establishes the correctness of the reduction ACM2 -> BI *)
+(** This establishes the correctness of the reduction 2-ACM -> LBI *)
 Theorem acm2_to_BI_correctness (loc : Set) Σ x y (p : loc) :
     acm2_accept Σ x y p
   ↔ LBI_provable BI_cut_free (BI_list_mult (acm2_ctx_to_BI Σ (map (@acm2_instr_src _) Σ) x y)) £(inl p).
